MirrorCharge!/src/MirrorCharge/Java/TestQuantPull.v
@@ -1,17 +1,28 @@
 Require Import MirrorCharge.Java.JavaType.
 Require Import MirrorCharge.Java.JavaFunc.
-Require Import MirrorCharge.RTac.PullQuant.
+
+Require Import MirrorCharge.SetoidRewrite.Base.
+Require Import MirrorCharge.SetoidRewrite.ILSetoidRewrite.
+Require Import MirrorCharge.SetoidRewrite.BILSetoidRewrite.
+Require Import MirrorCharge.SetoidRewrite.EmbedSetoidRewrite.
+
+Require Import MirrorCharge.PullQuant.BILPullQuant.
+Require Import MirrorCharge.PullQuant.ILPullQuant.
+Require Import MirrorCharge.PullQuant.EmbedPullQuant.
 
 Require Import MirrorCharge.ModularFunc.BaseFunc.
 Require Import MirrorCharge.ModularFunc.ILogicFunc.
+Require Import MirrorCharge.ModularFunc.EmbedFunc.
 
 Require Import MirrorCore.Lambda.ExprCore.
 
-Definition quant_pull := @quant_pull typ func _ _ _ (fun _ => true).
-Definition rewrite_exs := @rewrite_exs typ func _ _ (fun _ => true).
+Definition pull_quant := 
+	setoid_rewrite fEntails 
+		(sr_combine il_respects (sr_combine bil_respects embed_respects)) 
+		(sr_combine (il_match_plus (fun _ => true)) (sr_combine bil_match_plus eil_match_plus)).
 
  Definition goal : expr typ func :=
- 	mkAnd tyProp (mkTrue tyProp) (mkExists tyNat tyProp (mkEq tyNat (Var 0) (mkNat 3))).
+ 	mkAnd tyProp (mkTrue tyProp) (mkEmbed tyProp tyProp (mkExists tyNat tyProp (mkEq tyNat (Var 0) (Var 0)))).
 
 Fixpoint crazy_goal n :=
 	match n with
@@ -19,4 +30,6 @@ Fixpoint crazy_goal n :=
 		| S n => mkAnd tyProp (crazy_goal n) (crazy_goal n)
 	end.
 
-Time Eval vm_compute in quant_pull tyProp (crazy_goal 2).
+Set Printing Width 140.
+
+Time Eval vm_compute in pull_quant tyProp (crazy_goal 2).
