MirrorCharge!/src/MirrorCharge/PullQuant/EmbedPullQuant.v
@@ -1,0 +1,40 @@
+Require Import MirrorCore.Lambda.ExprCore.
+Require Import MirrorCore.Lambda.Red.
+Require Import MirrorCore.Lambda.ExprLift.
+Require Import MirrorCore.TypesI.
+
+Require Import ExtLib.Core.RelDec.
+
+Require Import MirrorCharge.SetoidRewrite.Base.
+Require Import MirrorCharge.ModularFunc.ILogicFunc.
+Require Import MirrorCharge.ModularFunc.EmbedFunc.
+Require Import MirrorCharge.AutoSetoidRewrite.
+
+Require Import Charge.Logics.ILogic.
+
+Section EILPullQuant.
+  Context {typ func : Type} {HIL : ILogicFunc typ func} {HB : EmbedFunc typ func}.
+  Context {RType_typ : RType typ}.
+  Context {RelDec_func : RelDec (@eq (expr typ func))}.
+
+  Let Rbase := expr typ func.
+
+Definition eil_match_plus (e : expr typ func) (_ : list (RG (expr typ func))) (rg : RG Rbase) : m (expr typ func) :=
+  match e with
+    | App a (App b P) =>
+      let P := beta (App P (Var 0)) in
+      match embedS (typ := typ) (func := expr typ func) a, ilogicS b with 
+      	| Some (eilf_embed u v), Some (ilf_exists t l) =>
+	      rg_plus
+	      (rg_bind (unifyRG (@rel_dec (expr typ func) _ _) rg (RGflip (RGinj (fEntails l))))
+	        (fun _ => rg_ret (mkExists t v (mkEmbed u v P))))
+	      (rg_bind (unifyRG (@rel_dec (expr typ func) _ _) rg (RGinj (fEntails l)))
+	        (fun _ => rg_ret (mkExists t v (mkEmbed u v P))))
+	    | _, _ => rg_fail
+	  end
+	| _ => rg_fail
+  end.
+
+End EILPullQuant.
+
+Implicit Arguments eil_match_plus [[typ] [func] [HIL] [HB] [RelDec_func]].
