MirrorCharge!/src/MirrorCharge/PullQuant/ILPullQuant.v
@@ -1,0 +1,87 @@
+Require Import MirrorCore.Lambda.ExprCore.
+Require Import MirrorCore.Lambda.Red.
+Require Import MirrorCore.Lambda.ExprLift.
+Require Import MirrorCore.TypesI.
+
+Require Import ExtLib.Core.RelDec.
+
+Require Import MirrorCharge.SetoidRewrite.Base.
+Require Import MirrorCharge.ModularFunc.BaseFunc.
+Require Import MirrorCharge.ModularFunc.ILogicFunc.
+Require Import MirrorCharge.AutoSetoidRewrite.
+
+Require Import Charge.Logics.ILogic.
+
+Section ILPullQuant.
+  Context {typ func : Type} {HIL : ILogicFunc typ func} {HB : BaseFunc typ func}.
+  Context {RType_typ : RType typ}.
+  Context {RelDec_func : RelDec (@eq (expr typ func))}.
+
+  Let Rbase := expr typ func.
+
+  Variable inhabited : typ -> bool.  
+  Variable inhabited_sound : forall t, inhabited t = true -> Inhabited (typD t).
+
+Definition il_match_plus_l (e : expr typ func) (_ : list (RG (expr typ func))) (rg : RG Rbase) : m (expr typ func) :=
+  match e with
+    | App (App a (App b P)) Q =>
+      let P := beta (App P (Var 0)) in
+      let Q := lift 0 1 Q in
+      match ilogicS (typ := typ) (func := expr typ func) a, ilogicS b with 
+      	| Some (ilf_and _), Some (ilf_exists t l) =>
+	      rg_plus
+	      (rg_bind (unifyRG (@rel_dec (expr typ func) _ _) rg (RGflip (RGinj (fEntails l))))
+	        (fun _ => rg_ret (mkExists t l (mkAnd l P Q))))
+	      (rg_bind (unifyRG (@rel_dec (expr typ func) _ _) rg (RGinj (fEntails l)))
+	        (fun _ => rg_ret (mkExists t l (mkAnd l P Q))))
+      	| Some (ilf_or _), Some (ilf_exists t l) =>
+      	  let rewrite_rl :=
+	        rg_bind (unifyRG (@rel_dec (expr typ func) _ _) rg (RGflip (RGinj (fEntails l))))
+		      (fun _ => rg_ret (mkExists t l (mkOr l P Q))) in
+			if inhabited t then
+		      rg_plus 
+		        rewrite_rl 
+		        (rg_bind (unifyRG (@rel_dec (expr typ func) _ _) rg (RGinj (fEntails l)))
+		          (fun _ => rg_ret (mkExists t l (mkOr l P Q))))
+		    else
+		      rewrite_rl
+	    | _, _ => rg_fail
+	  end
+	| _ => rg_fail
+  end.
+  
+Definition il_match_plus_r (e : expr typ func) (_ : list (RG (expr typ func))) (rg : RG Rbase) : m (expr typ func) :=
+  match e with
+   | App (App a P) (App b Q) =>
+   	 let P := lift 0 1 P in
+   	 let Q := beta (App Q (Var 0)) in
+     match ilogicS a, ilogicS b with
+       | Some (ilf_and _), Some (ilf_exists t l) =>
+	      rg_plus
+	        (rg_bind
+	          (unifyRG (@rel_dec (expr typ func) _ _ ) rg (RGinj (fEntails l)))
+	            (fun _ => rg_ret (mkExists t l (mkAnd l P Q))))
+  	        (rg_bind
+	          (unifyRG (@rel_dec (expr typ func) _ _) rg (RGflip (RGinj (fEntails l))))
+	            (fun _ => rg_ret (mkExists t l (mkAnd l P Q))))
+       | Some (ilf_or _), Some (ilf_exists t l) =>
+         let rewrite_rl := 
+		   rg_bind (unifyRG (@rel_dec (expr typ func) _ _) rg (RGflip (RGinj (fEntails l))))
+		     (fun _ => rg_ret (mkExists t l (mkOr l P Q))) in
+		   if inhabited t then
+		     rg_plus
+		       rewrite_rl
+		       (rg_bind (unifyRG (@rel_dec (expr typ func) _ _ ) rg (RGinj (fEntails l)))
+		         (fun _ => rg_ret (mkExists t l (mkOr t P Q))))
+		   else
+		     rewrite_rl
+	   | _, _ => rg_fail
+	 end
+   | _ => rg_fail
+ end.
+
+Definition il_match_plus := sr_combine il_match_plus_l il_match_plus_r.
+
+End ILPullQuant.
+
+Implicit Arguments il_match_plus [[typ] [func] [HIL] [RelDec_func]].
