MirrorCharge!/src/MirrorCharge/SetoidRewrite/Base.v
@@ -1,0 +1,93 @@
+Require Import MirrorCore.Lambda.ExprCore.
+Require Import MirrorCore.Lambda.ExprD.
+Require Import MirrorCore.Lambda.Red.
+Require Import MirrorCore.Lambda.ExprLift.
+Require Import MirrorCore.TypesI.
+Require Import MirrorCore.SymI.
+Require Import MirrorCore.ExprI.
+
+Require Import ExtLib.Core.RelDec.
+Require Import ExtLib.Data.Fun.
+Require Import ExtLib.Data.Nat.
+Require Import ExtLib.Tactics.
+Require Import MirrorCore.syms.SymSum.
+
+Require Import MirrorCharge.AutoSetoidRewrite.
+
+Set Implicit Arguments.
+Set Strict Implicit.
+
+Section SetoidRewrite.
+  Context {typ func : Type}.
+
+  Context {RType_typ : RType typ} {RelDec_typ_eq : RelDec (@eq typ)}
+          {RelDecCorrect_typ_eq : RelDec_Correct RelDec_typ_eq}.
+          
+  Context {RelDec_func_eq : RelDec (@eq (expr typ func))}.
+
+  Let Rbase := expr typ func.
+
+  Definition m (T : Type) : Type :=
+    rsubst Rbase -> option (T * rsubst Rbase).
+
+  Definition rg_bind {T U} (a : m T) (b : T -> m U) : m U :=
+    fun s => match a s with
+               | None => None
+               | Some (val,s') => b val s'
+             end.
+  Definition rg_fail {T} : m T := fun _ => None.
+  Definition rg_ret {T} (v : T) : m T := fun s => Some (v, s).
+  Definition rg_plus {T} (l r : m T) : m T :=
+    fun s =>
+      let v := l s in
+      match v with
+        | None => r s
+        | Some _ => v
+      end.
+		
+  Definition rw_type := expr typ func -> list (RG (expr typ func))
+                        -> RG (expr typ func) -> m (expr typ func).
+
+  Section interleave.
+    Variables (rw rw' : rw_type -> rw_type).
+
+    Fixpoint interleave (n : nat)
+             (e : expr typ func) (rvars : list (RG (expr typ func)))
+             (rg : RG (expr typ func)) : m (expr typ func) :=
+      match n with
+        | 0 => rg_fail
+        | S n => rw (fun rs => rw' (fun e rvars rg rs => interleave n e rvars rg rs) rs) e rvars rg
+      end.
+  End interleave.
+
+  Fixpoint rw_fix (n : nat)
+    (rw : rw_type -> rw_type)
+    (e : expr typ func) (rvars : list (RG Rbase)) (rg : RG Rbase)
+    (rs : rsubst Rbase) : option (expr typ func * rsubst Rbase) :=
+    match n with
+      | 0 => Some (e,rs)
+      | S n => rw (fun e rvars rg rs => rw_fix n rw e rvars rg rs) e rvars rg rs
+    end.
+
+  Definition sr_combine (f g : expr typ func -> list (RG (expr typ func)) -> RG (expr typ func) -> m (expr typ func))
+    (e : (expr typ func)) (rvars : list (RG (expr typ func))) (rg : RG (expr typ func)) :
+  	m (expr typ func) :=
+    rg_plus (f e rvars rg) (g e rvars rg).
+
+  Variable rel : typ -> Rbase.
+  Variable rewrite_respects : Rbase -> list (RG Rbase) -> RG Rbase -> m (expr typ func).
+  Variable rewrite_exs : Rbase -> list (RG Rbase) -> RG Rbase -> m (expr typ func).
+
+  Definition setoid_rewrite (l : typ) (e : expr typ func) : expr typ func :=
+    match
+      rw_fix 500 (@setoid_rewrite typ func (expr typ func)
+                       rel_dec
+                       rewrite_exs rewrite_respects)
+        e nil (RGinj (rel l))
+        (rsubst_empty _)
+    with
+      | None => e
+      | Some (e,_) => e
+    end.
+  
+End SetoidRewrite.
