MirrorCharge!/src/MirrorCharge/SetoidRewrite/ILSetoidRewrite.v
@@ -1,0 +1,49 @@
+Require Import MirrorCore.Lambda.ExprCore.
+
+Require Import ExtLib.Core.RelDec.
+
+Require Import MirrorCharge.SetoidRewrite.Base.
+Require Import MirrorCharge.ModularFunc.BaseFunc.
+Require Import MirrorCharge.ModularFunc.ILogicFunc.
+Require Import MirrorCharge.AutoSetoidRewrite.
+
+Section ILSetoidRewrite.
+	Context {typ func : Type} {HIL : ILogicFunc typ func} {HB : BaseFunc typ func}.
+	Context {RelDec_func : RelDec (@eq (expr typ func))}.
+
+	Let Rbase := expr typ func.
+
+  Definition il_respects (e : Rbase) (_ : list (RG Rbase))
+	   (rg : RG Rbase) : m (expr typ func) :=
+	   match ilogicS (typ := typ) (func := expr typ func) e with
+		 | Some (ilf_and l) => 
+		 	 rg_bind (unifyRG (@rel_dec (expr typ func) _ _) rg 
+			         (RGrespects (RGinj (fEntails l)) 
+			         (RGrespects (RGinj (fEntails l)) 
+			         (RGinj (fEntails l)))))
+				 (fun _ => rg_ret (fAnd l))
+		 | Some (ilf_or l) => 
+			 rg_bind (unifyRG (@rel_dec (expr typ func) _ _) rg 
+			         (RGrespects (RGinj (fEntails l)) 
+			         (RGrespects (RGinj (fEntails l))
+			         (RGinj (fEntails l)))))
+				 (fun _ => rg_ret (fOr l))
+		 | Some (ilf_impl l) => 
+			 rg_bind (unifyRG (@rel_dec (expr typ func) _ _) rg 
+			                  (RGrespects (RGflip (RGinj (fEntails l))) 
+			                  (RGrespects (RGinj (fEntails l)) 
+			                  (RGinj (fEntails l)))))
+				 (fun _ => rg_ret (fImpl l))
+		 | Some (ilf_exists t l) => 
+			 rg_bind (unifyRG (@rel_dec (expr typ func) _ _) rg 
+			                  (RGrespects (RGrespects (RGinj (fEq t))
+				 	 	                              (RGinj (fEntails l)))
+						                  (RGinj (fEntails l))))
+						                 
+				 (fun _ => rg_ret (fExists t l))
+		 | Some (ilf_true l) => rg_bind (unifyRG (@rel_dec (expr typ func) _ _) rg (RGinj (fEntails l)))
+			 	(fun _ => rg_ret (fTrue l))
+		 | _ => rg_fail
+	 end.
+
+End ILSetoidRewrite.
